powerpc/Asmgen.v
@@ -582,6 +582,7 @@ Definition transl_op
       do r1 <- ireg_of a1; do r2 <- ireg_of a2; do r <- freg_of res;
       OK (Pfmake r r1 r2 :: k)
   | Omakelong, a1 :: a2 :: nil =>
+      assertion Archi.ppc64;
       do r1 <- ireg_of a1; do r2 <- ireg_of a2; do r <- ireg_of res; OK (Plmake r r1 r2 :: k)
   | Olowlong, a1 :: nil =>
       assertion (mreg_eq a1 res);
@@ -592,83 +593,110 @@ Definition transl_op
       transl_cond_op cmp args res k
 (*c PPC64 operations *)
   | Olongconst n, nil =>
+      assertion Archi.ppc64;
       do r <- ireg_of res; OK (loadimm64 r n k)
   | Ocast32signed, a1 :: nil =>
+      assertion Archi.ppc64;
       do r1 <- ireg_of a1; do r <- ireg_of res;
       OK (Pextsw r r1 :: k)
   | Ocast32unsigned, a1 :: nil =>
+      assertion Archi.ppc64;
       do r1 <- ireg_of a1; do r <- ireg_of res;
       OK (Pextzw r r1 :: k)
   | Oaddl, a1 :: a2 :: nil =>
+      assertion Archi.ppc64;
       do r1 <- ireg_of a1; do r2 <- ireg_of a2; do r <- ireg_of res;
       OK (Padd64 r r1 r2 :: k)
   | Oaddlimm n, a1 :: nil =>
+      assertion Archi.ppc64;
       do r1 <- ireg_of a1; do r <- ireg_of res;
       OK (addimm64 r r1 n k)
   | Osubl, a1 :: a2 :: nil =>
+      assertion Archi.ppc64;
       do r1 <- ireg_of a1; do r2 <- ireg_of a2; do r <- ireg_of res;
       OK (Psubfc64 r r2 r1 :: k)
   | Onegl, a1 :: nil =>
+      assertion Archi.ppc64;
       do r1 <- ireg_of a1; do r <- ireg_of res;
       OK (Psubfic64 r r1 Int64.zero :: k)
   | Omull, a1 :: a2 :: nil =>
+      assertion Archi.ppc64;
       do r1 <- ireg_of a1; do r2 <- ireg_of a2; do r <- ireg_of res;
       OK (Pmulld r r1 r2 :: k)
   | Omullhs, a1 :: a2 :: nil =>
+      assertion Archi.ppc64;
       do r1 <- ireg_of a1; do r2 <- ireg_of a2; do r <- ireg_of res;
         OK (Pmulhd r r1 r2 :: k)
   | Omullhu, a1 :: a2 :: nil =>
+      assertion Archi.ppc64;
       do r1 <- ireg_of a1; do r2 <- ireg_of a2; do r <- ireg_of res;
         OK (Pmulhdu r r1 r2 :: k)
   | Odivl, a1 :: a2 :: nil =>
+      assertion Archi.ppc64;
       do r1 <- ireg_of a1; do r2 <- ireg_of a2; do r <- ireg_of res;
       OK (Pdivd r r1 r2 :: k)
   | Odivlu, a1 :: a2 :: nil =>
+      assertion Archi.ppc64;
       do r1 <- ireg_of a1; do r2 <- ireg_of a2; do r <- ireg_of res;
       OK (Pdivdu r r1 r2 :: k)
   | Oandl,  a1 :: a2 :: nil =>
+      assertion Archi.ppc64;
       do r1 <- ireg_of a1; do r2 <- ireg_of a2; do r <- ireg_of res;
       OK (Pand_64 r r1 r2 :: k)
   | Oandlimm n, a1 :: nil =>
+      assertion Archi.ppc64;
       do r1 <- ireg_of a1; do r <- ireg_of res;
       OK (andimm64 r r1 n k)
   | Oorl,  a1 :: a2 :: nil =>
+      assertion Archi.ppc64;
       do r1 <- ireg_of a1; do r2 <- ireg_of a2; do r <- ireg_of res;
       OK (Por64 r r1 r2 :: k)
   | Oorlimm n, a1 :: nil =>
+      assertion Archi.ppc64;
       do r1 <- ireg_of a1; do r <- ireg_of res;
       OK (orimm64 r r1 n k)
   | Oxorl,  a1 :: a2 :: nil =>
+      assertion Archi.ppc64;
       do r1 <- ireg_of a1; do r2 <- ireg_of a2; do r <- ireg_of res;
       OK (Pxor64 r r1 r2 :: k)
   | Oxorlimm n, a1 :: nil =>
+      assertion Archi.ppc64;
       do r1 <- ireg_of a1; do r <- ireg_of res;
       OK (xorimm64 r r1 n k)
   | Onotl, a1 :: nil =>
+      assertion Archi.ppc64;
       do r1 <- ireg_of a1; do r <- ireg_of res;
       OK (Pnor64 r r1 r1 :: k)
   | Oshll, a1 :: a2 :: nil =>
+      assertion Archi.ppc64;
       do r1 <- ireg_of a1; do r2 <- ireg_of a2; do r <- ireg_of res;
       OK (Psld r r1 r2 :: k)
   | Oshrl, a1 :: a2 :: nil =>
+      assertion Archi.ppc64;
       do r1 <- ireg_of a1; do r2 <- ireg_of a2; do r <- ireg_of res;
       OK (Psrad r r1 r2 :: k)
   | Oshrlimm n, a1 :: nil =>
+      assertion Archi.ppc64;
       do r1 <- ireg_of a1; do r <- ireg_of res;
       OK (Psradi r r1 n :: k)
   | Oshrlu, a1 :: a2 :: nil =>
+      assertion Archi.ppc64;
       do r1 <- ireg_of a1; do r2 <- ireg_of a2; do r <- ireg_of res;
       OK (Psrd r r1 r2 :: k)
   | Orolml amount mask, a1 :: nil =>
+      assertion Archi.ppc64;
       do r1 <- ireg_of a1; do r <- ireg_of res;
       OK (rolm64 r r1 amount mask k)
   | Oshrxlimm n, a1 :: nil =>
+      assertion Archi.ppc64;
       do r1 <- ireg_of a1; do r <- ireg_of res;
       OK (Psradi r r1 n :: Paddze64 r r :: k)
   | Olongoffloat, a1 :: nil =>
+      assertion Archi.ppc64;
       do r1 <- freg_of a1; do r <- ireg_of res;
       OK (Pfctid r r1 :: k)
   | Ofloatoflong, a1 :: nil =>
+      assertion Archi.ppc64;
       do r1 <- ireg_of a1; do r <- freg_of res;
       OK (Pfcfl r r1 :: k)
   | _, _ =>
@@ -749,6 +777,7 @@ Definition transl_load (chunk: memory_chunk) (addr: addressing)
       do r <- ireg_of dst;
       transl_memory_access (Plwz r) (Plwzx r) addr args GPR12 k
   | Mint64 =>
+      assertion Archi.ppc64;
       do r <- ireg_of dst;
       transl_memory_access (Pld r) (Pldx r) addr args GPR12 k
   | Mfloat32 =>
@@ -775,6 +804,7 @@ Definition transl_store (chunk: memory_chunk) (addr: addressing)
       do r <- ireg_of src;
       transl_memory_access (Pstw r) (Pstwx r) addr args temp k
   | Mint64  =>
+      assertion Archi.ppc64;
       do r <- ireg_of src;
       transl_memory_access (Pstd r) (Pstdx r) addr args temp k
   | Mfloat32 =>
